Ajout balise

src/CoqNom/src/Formalisation/ZeroCopy/Definition.v
@@ -5,14 +5,19 @@ Require Import Vector.
 From Equations Require Import Equations.
 Import disjoint.
 
+(* =Bit= *)
 Definition Bit := bool.
+(* =end= *)
 
+(* =ValuesFormat= *)
 Class ValuesFormat (X : Type) :=
   mk_values {
       size : nat;
       encode : X -> Vector.t Bit size;
       decode : Vector.t Bit size -> option X;
       spec : forall (x : X), decode (encode x) = Some x; }.
+(* =end= *)
+
 
 Local Instance ValuesBool : ValuesFormat bool.
 refine (mk_values bool 1
@@ -24,15 +29,19 @@ refine (mk_values bool 1
 intros. reflexivity.
 Defined.
 
+(* =Etiquette= *)
 Class Etiquette `{Countable etiquette} :=
   mk_etiquette {
       set_etiquette : gset etiquette;
       set_etiquette_spec: forall (e : etiquette), e ∈ set_etiquette; }.
+(* =end= *)
 
+(* =Result= *)
 Inductive Result :=
 | Value : forall `{ValuesFormat X}, X -> Result
 | Span : span -> Result
 | Struct : forall `{Etiquette etiquette}, (etiquette -> Result) -> Result.
+(* =end= *)
 
 Arguments Value [X _].
 Arguments Struct [etiquette _ _ _].
@@ -47,49 +56,64 @@ Fixpoint Result_to_list (t: Result) : list span :=
       list.foldr (fun eti r => Result_to_list (st eti) ++ r) [] list_etiquette
   end.
 
+(* =Decodeur= *)
 Definition Decodeur := span -> option Result.
+(* =end= *)
 
 Open Scope N_scope.
 
-Definition set_span (s : span) := inject (pos s) (pos s + len s).
-
+(* =scope_in= *)
 Definition scope_in (s t : span) := set_span s ⊆ set_span t.
+(* =end= *)
 
+(* =ResultWeakZC= *)
 Fixpoint ResultWeakZC (s : span) (r : Result) : Prop :=
   match r with
   | Value _ => True
   | Span v => scope_in v s
   | Struct ft => forall e, ResultWeakZC s (ft e)
   end.
+(* =end= *)
 
-Definition DecodeurWeakZC (d: Decodeur) :=
-  forall s ft,
-    d s = Some ft ->
-    ResultWeakZC s ft.
+(* =DecodeurWeakZC= *)
+Definition DecodeurWeakZC (d: Decodeur) := forall s ft,
+    d s = Some ft -> ResultWeakZC s ft.
+(* =end= *)
 
+(* =ResultZC= *)
 Fixpoint ResultZC (s : span) (r : Result) : Prop :=
   match r with
   | Value _ => False
   | Span v => scope_in v s
   | Struct ft => forall e, ResultZC s (ft e)
   end.
+(* =end= *)
 
-Definition DecodeurZC (d : Decodeur) :=
-  forall s ft,
-    d s = Some ft ->
-    ResultZC s ft.
+(* =DecodeurZC= *)
+Definition DecodeurZC (d : Decodeur) := forall s ft,
+    d s = Some ft -> ResultZC s ft.
+(* =end= *)
 
 (** Version tous les spans de la structures sont disjointes deux à deux **)
 
-Definition Result_safe (r : Result) : Prop :=
-  forall s t, s <> t -> s ∈ Result_to_list r -> t ∈ Result_to_list r -> disjoint s t.
+(* =Result_safe= *)
+Definition Result_safe (r : Result) : Prop := forall s t,
+    s <> t ->
+    s ∈ Result_to_list r ->
+    t ∈ Result_to_list r ->
+    disjoint s t.
+(* =end= *)
 
 (** Version SL **)
 
+(* =Result_safeSL= *)
 Definition Result_safeSL (r : Result) : iProp :=
   [∗ list] v ∈ Result_to_list r, IsFresh v.
+(* =end= *)
 
+(* =safe_bridge= *)
 Theorem safe_bridge : forall (r : Result), Result_safeSL r ⊢ ⌜ Result_safe r ⌝.
+(* =end= *)
 Proof.
   unfold Result_safe. induction r; simpl; intros.
   - iIntros "HA". iPureIntro. intros s t NEQ F. inversion F.
@@ -107,5 +131,6 @@ Proof.
     + iClear "HA". iApply (IsFresh_spec with "Hs Ht").
 Qed.
 
+(* =DecodeurZC_safe= *)
 Definition DecodeurZC_safe (d : Decodeur) :=
   forall s ft, d s = Some ft -> Result_safe ft.
